MLIR/Semantics/Refinement.lean
@@ -1,0 +1,138 @@
+/-
+## Refinement
+
+This file defines the definition of a refinement.
+For now, this is only defined for the arith dialect, but this 
+can hopefully be defined for arbitrary semantics.
+-/
+
+import MLIR.Semantics.Semantics
+import MLIR.Dialects.ArithSemantics
+import MLIR.Semantics.UB
+open MLIR.AST
+
+def SSAEnv.refinement (env1 env2: SSAEnv arith) : Prop :=
+  ∀ v val, env2.getT v = some val -> env1.getT v = some val
+
+-- One SSA environment is a refinement of the other if all variables
+-- defined in the environment are also defined by the other first one.
+-- If the SSA environment is none (corresponding to an UB), then we have
+-- a refinement for all other possible SSA environment, or UB 
+def refinement (env1 env2: Option R × SSAEnv arith) : Prop :=
+  match env1, env2 with
+  | (none, _), _ => True
+  | (some r1, env1), (some r2, env2) =>
+    r1 = r2 ∧ SSAEnv.refinement env1 env2
+  | _, _ => False
+
+theorem SSAEnv.refinement_set :
+    refinement env1 env2 ->
+    refinement (SSAEnv.set name τ val env1) (SSAEnv.set name τ val env2) := by
+  simp [refinement, SSAEnv.refinement]
+  intros Href name' val' Hget
+  byCases H: name = name'
+  . rw [SSAEnv.getT_set_eq] <;> try assumption
+    rw [SSAEnv.getT_set_eq] at Hget <;> assumption
+  . rw [SSAEnv.getT_set_ne] <;> try assumption
+    rw [SSAEnv.getT_set_ne] at Hget <;> try assumption
+    apply Href
+    assumption
+
+theorem arithRefinement:
+    ∀ (env1 env2: SSAEnv arith),
+    SSAEnv.refinement env1 env2 ->
+    ∀ (res: Option SSAVal) (op: Op arith) (t: Fitree (SSAEnvE arith +' Semantics.E arith) _),
+    Semantics.semantics_op res op = some t ->
+    refinement (run (Fitree.translate Member.inject t) env1) (run (Fitree.translate Member.inject t) env2) := by
+  intros env1 env2 Href res op t Hsem
+  simp [Semantics.semantics_op, arith_semantics_op] at Hsem
+  split at Hsem
+  . split at Hsem <;> try contradiction
+    split at Hsem <;> try contradiction
+    split at Hsem <;> try contradiction
+    simp at Hsem
+    rw [←Hsem]
+    cases res with
+    | none =>
+      simp_itree; simp [run]; simp_itree; simp [refinement]
+      assumption
+    | some val =>
+      simp_itree
+      simp [run]
+      simp_itree
+      simp [refinement] at *
+      apply SSAEnv.refinement_set <;> try assumption
+  . split at Hsem <;> try contradiction
+    split at Hsem <;> try contradiction
+    split at Hsem <;> try contradiction
+    simp at Hsem
+    sorry
+  . sorry
+  . sorry
+  -- cases op with | mk name args bbs regions attrs ty => 
+  
+  
+
+
+
+section ArithPreservation
+variable [Hsem: Semantics arith]
+
+variable (HCorrectsem:
+           ∀ (env1 env2: SSAEnv arith),
+           SSAEnv.refinement env1 env2 ->
+           ∀ (res: Option SSAVal) (op: Op arith) (t: Fitree (SSAEnvE arith +' Semantics.E arith) _),
+           Semantics.semantics_op res op = some t ->
+           refinement (run (Fitree.translate Member.inject t) env1) (run (Fitree.translate Member.inject t) env2))
+
+mutual
+theorem arithPreservesRefinementOp :
+  ∀ (env1 env2: SSAEnv arith),
+    SSAEnv.refinement env1 env2 ->
+    ∀ (res: Option SSAVal) (op: Op arith),
+    refinement (run (semantics_op! res op) env1) (run (semantics_op! res op) env2) := by
+  intros env1 env2 Href res op
+  simp [semantics_op!, Semantics.semantics_op]
+  cases Ht: (Semantics.semantics_op (self := Hsem) res op)
+  . simp [run, interp_ub, interp]
+    simp_itree
+    simp [refinement]
+  . simp
+    apply HCorrectsem <;> assumption
+
+theorem arithPreservesRefinementBBStmt :
+  ∀ (env1 env2: SSAEnv arith),
+    SSAEnv.refinement env1 env2 ->
+    ∀ (prog: BasicBlockStmt arith),
+    refinement (run ⟦prog⟧ env1) (run ⟦prog⟧ env2) := by
+  intros env1 env2 Href prog
+  cases prog <;> apply arithPreservesRefinementOp _ _ Href
+end
+
+end ArithPreservation
+
+
+section ArithPreservation'
+mutual
+theorem arithPreservesRefinementOp' :
+  ∀ (env1 env2: SSAEnv arith),
+    SSAEnv.refinement env1 env2 ->
+    ∀ (res: Option SSAVal) (op: Op arith),
+    refinement (run (S:=arithSemantics) (semantics_op! (S:=arithSemantics) res op) env1) (run (S:=arithSemantics) (semantics_op! (S:=arithSemantics) res op) env2) := by
+  intros env1 env2 Href res op
+  simp [semantics_op!, Semantics.semantics_op]
+
+theorem arithPreservesRefinementBBStmt' :
+  ∀ (env1 env2: SSAEnv arith),
+    SSAEnv.refinement env1 env2 ->
+    ∀ (prog: BasicBlockStmt arith),
+    refinement (run (S:=arithSemantics) (Denote.denote (S:=arithSemantics) prog) env1) (run (S:=arithSemantics) (Denote.denote (S:=arithSemantics) prog) env2) := by
+  intros env1 env2 Href prog
+  cases prog 
+  . simp [Denote.denote, semantics_bbstmt]
+    sorry
+  . sorry
+  --cases prog <;> apply arithPreservesRefinementOp' _ _ Href
+end
+
+end ArithPreservation'
